Roolean/QfBv/Domain.lean
@@ -35,6 +35,11 @@ public inductive BiReductionOp
   | Sle
 deriving Repr, Inhabited
 
+public inductive ExtOp
+  | Uext
+  | Sext
+deriving Repr, Inhabited
+
 public class Domain (α: Nat → Type) where
   ofBitvector {w}: Bitvector w → α w
   toBitvector? {w}: α w → Option (Bitvector w)
@@ -42,5 +47,6 @@ public class Domain (α: Nat → Type) where
   uniOp {w}: α w → UniOp → α w
   biNormal{w}: α w → α w → BiNormalOp → α w
   biReduction {w}: α w → α w → BiReductionOp → α 1
+  extOp {w}: α w → (m: Nat) → ExtOp → α m
 
   fmt {w}: α w → String
