Roolean/QfBv/Domain/Bitvector3/ExtOps.lean
@@ -1,0 +1,21 @@
+module
+
+public import Roolean.QfBv.Domain.Bitvector3.Basic
+import Roolean.QfBv.Domain.Bitvector3.BiNormalOps
+
+namespace Bitvector3
+
+ --- DEFINITIONS ---
+
+public def extOp {w} (domain: Bitvector3 w) (newWidth: Nat) (op: ExtOp) : Bitvector3 newWidth :=
+  match op with
+  | .Uext =>
+    sorry
+  | .Sext =>
+    sorry
+
+ --- THEOREMS ---
+
+public theorem extOp_sound {w} (a: Bitvector3 w) (c: Bitvector w) (m: Nat) (op: ExtOp)
+  : γ a c → γ (a.extOp m op) (c.extOp m op):= by
+  sorry
