Roolean/QfBv/Evaluator.lean
@@ -26,6 +26,10 @@ public def eval {v w} {α : Nat → Type} [Domain α]
       let right := eval right assignment
       Domain.biReduction left right op
 
+    | BvTerm.Extension inner newWidth op =>
+      let inner := eval inner assignment
+      Domain.extOp inner newWidth op
+
 public theorem eval_sound {w v} {α : Nat → Type} [Domain α] [AbstractDomain α]
   (f: BvTerm v w) (a: Assignment v α) (c: Assignment v Bitvector) (h: a.γ c)
   : AbstractDomain.γ (eval f a) (eval f c) := by
@@ -37,13 +41,11 @@ public theorem eval_sound {w v} {α : Nat → Type} [Domain α] [AbstractDomain 
   {
     -- variable
     rename_i i
-    simp[eval.eq_def]
     exact (Assignment.γ_elem a c i) h
   }
   {
     -- unary
     rename_i w pf op h
-    repeat rw[eval.eq_def]
     exact AbstractDomain.uniOp_sound (eval pf a) (eval pf c) op h
   }
   {
@@ -53,10 +55,15 @@ public theorem eval_sound {w v} {α : Nat → Type} [Domain α] [AbstractDomain 
       op (eval left c) (eval right c) h1 h2
   }
   {
-  -- binary reduction
+    -- binary reduction
     rename_i left right op h1 h2
     exact AbstractDomain.biReduction_sound (eval left a) (eval right a)
       op (eval left c) (eval right c) h1 h2
+  }
+  {
+    -- extension
+    rename_i inner m op h
+    exact AbstractDomain.extOp_sound (eval inner a) (eval inner c) m op h
   }
 
 def eval3bv {v} {α : Nat → Type} [Domain α]
